Proofs in-progress with definitions separated

lambdaE.lean
@@ -1,224 +1,44 @@
 import Lean
 
-namespace Definitions
-
-/-
-    A, B, Γ := int | ε | A → B | A & B | {l ∶ A}
-
-    Supporting literal init, unit (top), arrow, intersection and record types.
-    Note: Typing context Γ is unified with types, hence typing context Γ is simply a type.
--/
-inductive Typ : Type  where
-    | int     : Typ
-    | top     : Typ
-    | arr     : Typ → Typ → Typ
-    | and     : Typ → Typ → Typ
-    | rcd     : String → Typ → Typ
-
-/-
-    E := ? | i | ε | E₁ E₂ | E₁ ▷ E₂ | E₁ ,, E₂ | λA. E | E.i | ⟨v, λA. E⟩ | E.l
--/
-inductive Exp : Type where
-    | ctx     : Exp
-    | lit     : Nat → Exp
-    | unit    : Exp
-    | app     : Exp → Exp → Exp
-    | box     : Exp → Exp → Exp
-    | mrg     : Exp → Exp → Exp
-    | lam     : Typ → Exp → Exp
-    | proj    : Exp → Nat → Exp
-    | clos    : Exp → Typ → Exp → Exp
-    | erec    : String → Exp → Exp
-    | rproj   : Exp → String → Exp
-
-inductive Lookup : Typ → Nat → Typ → Prop where
-    | lzero :
-        ∀ A B,  Lookup (Typ.and A B) 0 B
-    | lsucc :
-        ∀ A B n C,  Lookup A n C →
-                    Lookup (Typ.and A B) (n + 1) C
-
-inductive Value : Exp → Prop where
-    | vint      :
-        ∀ n, Value (Exp.lit n)
-    | vunit     :
-        Value Exp.unit
-    | vclosl    :
-        ∀ v A e, Value v → Value (Exp.clos v A e)
-    | vrcd      :
-        ∀ l v, Value v → Value (Exp.erec l v)
-    | vmrg      :
-        ∀ v1 v2, Value v1 → Value v2 → Value (Exp.mrg v1 v2)
-
-inductive Lin : String → Typ → Prop where
-    | lin_rcd   :
-        ∀ A l, Lin l (Typ.rcd l A)
-    | lin_andl  :
-        ∀ A B l,
-            Lin l A → Lin l (Typ.and A B)
-    | lin_andr  :
-        ∀ A B l,
-        Lin l B →
-        Lin l (Typ.and A B)
-
-inductive RLookup : Typ → String → Typ → Prop where
-    | rlzero : ∀ l B, RLookup (Typ.rcd l B) l B
-    | landl : ∀ A B C l,
-        RLookup A l C →
-        ¬ Lin l B →
-        RLookup (Typ.and A B) l C
-    | landr : ∀ A B C l,
-        RLookup B l C →
-        ¬ Lin l A →
-        RLookup (Typ.and A B) l C
-
-inductive HasType : Typ → Exp → Typ → Prop where
-    | tctx      : ∀ E, HasType E Exp.ctx E
-    | tint      : ∀ E i, HasType E (Exp.lit i) Typ.int
-    | tunit     : ∀ E, HasType E Exp.unit Typ.top
-    | tapp      : ∀ E A B e1 e2,
-        HasType E e1 (Typ.arr A B)  →
-        HasType E e2 A              →
-        HasType E (Exp.app e1 e2) B
-    | tbox      : ∀ E A E1 e1 e2,
-        HasType E e1 E1 →
-        HasType E1 e2 A →
-        HasType E (Exp.box e1 e2) A
-    | tmrg      : ∀ E e1 e2 A B,
-        HasType E e1 A              →
-        HasType (Typ.and E A) e2 B  →
-        HasType E (Exp.mrg e1 e2) (Typ.and A B)
-    | tlam      : ∀ E A e B,
-        HasType (Typ.and E A) e B →
-        HasType E (Exp.lam A e) (Typ.arr A B)
-    | tproj     : ∀ E A e B n,
-        HasType E e A   →
-        Lookup A n B    →
-        HasType E (Exp.proj e n) B
-    | tclos     : ∀ E E1 A e ev B,
-        Value ev                    →
-        HasType Typ.top ev E1       →
-        HasType (Typ.and E1 A) e B  →
-        HasType E (Exp.clos ev A e) (Typ.arr A B)
-    | trcd      : ∀ E e A l,
-        HasType E e A  →
-        HasType E (Exp.erec l e) (Typ.rcd l A)
-    | trproj    : ∀ E e B l A,
-        HasType E e B →
-        RLookup B l A →
-        HasType E (Exp.rproj e l) A
-
-inductive LookupV : Exp → Nat → Exp → Prop where
-    | lvzero : ∀ v1 v2,
-        LookupV (Exp.mrg v1 v2) 0 v2
-    | lvsucc : ∀ v1 v2 n v3,
-        LookupV v1 n v3 →
-        LookupV (Exp.mrg v1 v2) (n + 1) v3
-
-inductive RLookupV : Exp → String → Exp → Prop where
-    | rvlzero   : ∀ l e,
-        RLookupV (Exp.erec l e) l e
-    | vlandl    : ∀ e1 e2 e l,
-        RLookupV e1 l e →
-        RLookupV (Exp.mrg e1 e2) l e
-    | vlandr    : ∀ e1 e2 e l,
-        RLookupV e2 l e →
-        RLookupV (Exp.mrg e1 e2) l e
-
-inductive Step : Exp → Exp → Exp → Prop where
-    | sctx : ∀ v,
-        Value v             →
-        Step v Exp.ctx v
-    | sblapp : ∀ v e1 e2 e1',
-        Value v             →
-        Step v e1 e1'       →
-        Step v (Exp.app e1 e2) (Exp.app e1' e2)
-    | sblbox : ∀ v e1 e2 e1',
-        Value v             →
-        Step v e1 e1'       →
-        Step v (Exp.box e1 e2) (Exp.box e1' e2)
-    | sblmrg : ∀ v e1 e2 e1',
-        Value v             →
-        Step v e1 e1'       →
-        Step v (Exp.mrg e1 e2) (Exp.mrg e1' e2)
-    | sbapp : ∀ v v1 e2 e2',
-        Value v             →
-        Value v1            →
-        Step v e2 e2'       →
-        Step v (Exp.app v1 e2) (Exp.app v1 e2')
-    | sbbox : ∀ v v1 e2 e2',
-        Value v             →
-        Value v1            →
-        Step v1 e2 e2'      →
-        Step v (Exp.box v1 e2) (Exp.box v1 e2')
-    | sbmrg : ∀ v v1 e' e,
-        Value v             →
-        Value v1            →
-        Step (Exp.mrg v v1) e e'    →
-        Step v (Exp.mrg v1 e) (Exp.mrg v1 e')
-    | sclos : ∀ v A e,
-        Value v     →
-        Step v (Exp.lam A e) (Exp.clos v A e)
-    | sbetalam : ∀ v v1 v2 A e,
-        Value v     →
-        Value v1    →
-        Value v2    →
-        Step v (Exp.app (Exp.clos v2 A e) v1) (Exp.box (Exp.mrg v2 v1) e)
-    | sboxv : ∀ v v1 v2,
-        Value v     →
-        Value v1    →
-        Value v2    →
-        Step v (Exp.box v1 v2) v2
-    | sproj : ∀ v e1 e2 n,
-        Value v         →
-        Step v e1 e2    →
-        Step v (Exp.proj e1 n) (Exp.proj e2 n)
-    | sprojv : ∀ v n v1 v2,
-        Value v         →
-        Value v1        →
-        LookupV v1 n v2 →
-        Step v (Exp.proj v1 n) v2
-    | srec : ∀ v e1 e2 l,
-        Value v         →
-        Step v e1 e2    →
-        Step v (Exp.erec l e1) (Exp.erec l e2)
-    | srproj : ∀ v e1 e2 l,
-        Value v         →
-        Step v e1 e2    →
-        Step v (Exp.rproj e1 l) (Exp.rproj e2 l)
-    | srprojv : ∀ v l v1 v2,
-        Value v             →
-        Value v1            →
-        RLookupV v1 l v2    →
-        Step v (Exp.rproj v1 l) v2
-
-end Definitions
-
 open Definitions
 
 variable  {v        : Definitions.Exp}
 variable  {A E E'   : Definitions.Typ}
 
-theorem value_weaken :
+theorem value_weaken:
     ∀ E v A,
-        Definitions.HasType E v A →
-        ∀ E', Definitions.Value v →
-        Definitions.HasType E' v A :=
-    by  intro E v A H E' Hv
-        induction H generalizing E'
-        case tctx E'                =>  cases Hv
-        case tint E n               =>  exact HasType.tint E' n
-        case tunit E                =>  exact HasType.tunit E'
-        case tapp B e1 e2 A B h1 h2 =>  cases Hv
-        case tbox E A B e1 e2       =>  cases Hv
-        case tmrg E A B e1 e2       =>
-            apply HasType.tmrg
-            · cases Hv; apply e1; assumption
-            · cases Hv; apply e2; assumption
-        case tlam E A B e1 e2           =>  cases Hv
-        case tproj E A e B n            =>  cases Hv
-        case tclos E' E1' A' e' ev' B'  =>
-            cases Hv; apply HasType.tclos; repeat assumption
-        case trcd E e A l           =>
-            cases Hv; apply HasType.trcd; apply l; assumption
-        case trproj E e B l A       =>  cases Hv
+        HasType E v A →
+        ∀ E', Value v →
+        HasType E' v A :=
+    by  intro E v A H E' Hv <;> induction H generalizing E' <;> cases Hv
+        case tint E n                   =>  exact HasType.tint E' n
+        case tunit E                    =>  exact HasType.tunit E'
+        case tmrg E A B e1 e2           =>  apply HasType.tmrg; apply A; assumption; apply B; assumption
+        case tclos E' E1' A' e' ev' B'  =>  apply HasType.tclos; repeat assumption
+        case trcd E e A l               =>  apply HasType.trcd; apply A; assumption
+
+theorem lookupv_value:
+    ∀ v n v',   LookupV v n v'  →
+                Value v →
+                Value v' :=
+    by  intro v n v' Hl
+        induction Hl <;> intro Hv <;> cases Hv <;> try assumption
+        case lvsucc v1 v2 _  => apply v1; assumption
+
+theorem lookup_pres_ctx:
+    ∀ E n A,    Lookup E n A → ∀ v v',
+                LookupV v n v'  →
+                Value v         →
+                HasType top v E →
+                HasType E v' A  :=
+    by
+    intro E n A Hl
+    induction Hl <;> intro v v' Hlv Hv Ht
+    case lzero =>
+        try repeat cases Hlv <;> try repeat cases Hv <;> cases Ht
+        case tmrg A' A'' B' v H1 H2 H3 =>
+            apply value_weaken <;> assumption
+    case lsucc v1 v2 H H_inner  =>
+        try repeat cases Hlv <;> try repeat cases Hv <;> cases H_inner
+        case lvsucc v1 v2 Hv'   =>
+            sorry
